Here is the fully detailed summary for **Part 11 â€“ Using `sym.expand()` to Confirm Symbolic Equalities** for your Obsidian notes:

---

## ğŸ”“ Part 11 â€“ Using `sym.expand()` to Confirm Symbolic Equalities

### ğŸ“Œ Purpose

This part shows how `sym.expand()` can be used to **force symbolic expressions into a fully expanded form**, making it easier to verify whether two expressions are truly equal.

---

### ğŸ§ª Problem Recap

Sometimes SymPy cannot directly evaluate:

$$ \text{Eq}(x^y \cdot x^z,\ x^{y+z}) $$

Even though mathematically valid, SymPy may **not return `True`** because of symbolic ambiguity.

---

### âœ… Step 1: Use `sym.expand(expr1 - expr2)`

```python
expr1 = x**y * x**z
expr2 = x**(y + z)

difference = sym.expand(expr1 - expr2)
```

If `difference == 0`, then:

$$ x^y \cdot x^z = x^{y+z} $$

---

### âœ… Step 2: Combine with `Eq()`

```python
sym.Eq(sym.expand(expr1 - expr2), 0)
```

Expected output:

$$ \text{True} $$

---

### ğŸ” What `expand()` Does

- Applies exponent and distributive rules
    
- Flattens expressions
    
- Makes structural comparison easier
    

---

### ğŸ§  Alternative: Compare Expanded Sides Directly

```python
sym.expand(expr1) == sym.expand(expr2)  # Returns True
```

This avoids using `Eq()` entirely and checks **Python-level equality** after expansion.

---

### ğŸ“Œ Example

```python
a = x**y * x**z
b = x**(y + z)

sym.expand(a - b)         # Returns 0
sym.Eq(sym.expand(a - b), 0)  # True
sym.expand(a) == sym.expand(b)  # True
```

---

### âœ… Summary Table

|Method|Code|Result|
|---|---|---|
|Expand diff|`sym.expand(expr1 - expr2)`|Should return `0`|
|Equation check|`Eq(expand(expr1 - expr2), 0)`|True|
|Compare both|`expand(expr1) == expand(expr2)`|True|

---

Would you like to continue with **Part 12 â€“ Using `sym.powsimp()` for Power-Specific Simplification**?