Here is the fully detailed summary for **Part 9 â€“ Understanding One-Argument Usage of `Eq()` with Default RHS = 0** for your Obsidian notes:

---

## âž– Part 9 â€“ Understanding One-Argument Usage of `Eq()` with Default RHS = 0

### ðŸ“Œ Purpose

This part explains how you can use `sym.Eq(expr)` with a **single argument**, and how SymPy interprets that by **automatically setting the right-hand side (RHS) to zero**.

---

### ðŸ§¾ Basic Usage

```python
sym.Eq(expr)
```

is equivalent to:

```python
sym.Eq(expr, 0)
```

It creates an equation like:

$$ \text{LHS} = 0 $$

---

### ðŸ§ª Example

```python
sym.Eq(x**2 - 9)
```

Is equivalent to:

$$ x^2 - 9 = 0 $$

You can verify:

```python
sym.Eq(x**2 - 9, 0)
```

---

### ðŸ”Ž Why This Works

SymPy treats the **missing RHS** as:

$$ \text{RHS} = 0 $$

which is helpful when you're checking whether an expression **equals zero**, or simplifying expressions for solving.

---

### ðŸ§  Conceptual Use Case

Given:

```python
lhs = 4
rhs = 2 + 2
```

Then:

```python
sym.Eq(lhs - rhs)
```

Will be:

$$ 4 - (2 + 2) = 0 \Rightarrow \text{True if simplified} $$

This setup helps **restate equations** in standard form:

$$ \text{(Left - Right)} = 0 $$

---

### ðŸ’¬ Checking Help: `shift + tab` or `?`

Inside Jupyter, placing your cursor in the function call and pressing `Shift + Tab` reveals:

```plaintext
Eq(lhs, rhs=0)
```

This confirms that the **default value** for `rhs` is `0`.

---

### âœ… Summary

|Syntax|Interpreted As|Output|
|---|---|---|
|`Eq(expr)`|`Eq(expr, 0)`|LHS = 0|
|`Eq(a - b)`|`a - b = 0`|Equation form|
|Help tip|`Shift + Tab`|Shows default arguments|

---

Would you like to continue with **Part 10 â€“ Limitations of Symbolic Equality (`Eq(expr1, expr2)` not returning `True`)**?